theories/Dot/stamping/skeleton.v
@@ -80,9 +80,9 @@ same_skel_vl (v1 v2: vl) {struct v1} : Prop :=
 with
 same_skel_dm (d1 d2: dm) {struct d1} : Prop :=
   match (d1, d2) with
-  | (dvl p1, dvl p2) => same_skel_path p1 p2
-  | (dvl _, _) => False
-  | (_, dvl _) => False
+  | (dpt p1, dpt p2) => same_skel_path p1 p2
+  | (dpt _, _) => False
+  | (_, dpt _) => False
     (* Only nontrivial cases. Could be replaced by a catchall. *)
   | (dtysyn _, dtysyn _) => True
   | (dtysyn _, dtysem _ _) => True
@@ -363,8 +363,8 @@ Qed.
 
 Lemma same_skel_dms_index_gen {ds ds' v l}:
   same_skel_dms ds ds' →
-  dms_lookup l ds = Some (dvl v) →
-  exists v', dms_lookup l ds' = Some (dvl v') ∧ same_skel_path v v'.
+  dms_lookup l ds = Some (dpt v) →
+  exists v', dms_lookup l ds' = Some (dpt v') ∧ same_skel_path v v'.
 Proof.
   revert ds' l v.
   induction ds as [|[lbl d] ds]; intros ds' l v Hds Hlu; simpl in *; first done.
@@ -387,11 +387,11 @@ Proof. elim: p p' => [v|p IHp l] [v'|p' l'] //=. naive_solver. Qed.
 
 Lemma same_skel_obj_lookup v v' p l:
   same_skel_vl v v' →
-  v @ l ↘ dvl p →
-  ∃ p', v' @ l ↘ dvl p' ∧ same_skel_tm (path2tm p) (path2tm p').
+  v @ l ↘ dpt p →
+  ∃ p', v' @ l ↘ dpt p' ∧ same_skel_tm (path2tm p) (path2tm p').
 Proof.
   intros Hv [ds [-> Hl]]. case: v' Hv => // ds' Hv.
-  have [p' [Hl' /same_skel_path2tm Hp]]: ∃ p', dms_lookup l (selfSubst ds') = Some (dvl p') ∧ same_skel_path p p'.
+  have [p' [Hl' /same_skel_path2tm Hp]]: ∃ p', dms_lookup l (selfSubst ds') = Some (dpt p') ∧ same_skel_path p p'.
   eapply (@same_skel_dms_index_gen (selfSubst ds)); by [|apply same_skel_dms_selfSubst].
   exists p'; split; by [|exists ds'].
 Qed.
