theories/Dot/typing/typingStamping.v
@@ -249,19 +249,19 @@ Section syntyping_stamping_lemmas.
         exact: (stamped_objIdent_subtype_mono _ Hts2)].
   - intros * Hus1 Hu1 IHs1 g.
     move: IHs1 => /(.$ g) /= [e1' [g1 ?]]; destruct_and!.
-    exists (dvl (pv (vabs e1'))), g1; split_and!;
+    exists (dpt (pv (vabs e1'))), g1; split_and!;
       repeat constructor; naive_solver.
   - intros * Hu1 IHs1 g.
     move: IHs1 => /(.$ g) /= [e1' [g1 ?]]; destruct_and!.
     have [v' ?]: ∃ v', e1' = tv v' by destruct e1'; naive_solver.
     simplify_eq/=; with_is_stamped inverse; with_is_unstamped inverse.
-    exists (dvl (pv v')), g1; naive_solver.
+    exists (dpt (pv v')), g1; naive_solver.
   - intros * Hu1 IHs1 Hus1 g.
     move: IHs1 => /(.$ g) /= [p1' [g1 ?]]; destruct_and!.
-    exists (dvl p1'), g1; naive_solver.
+    exists (dpt p1'), g1; naive_solver.
   - intros * Hu1 IHs1 Hus1 g.
     move: IHs1 => /(.$ g) /= [ds' [g1 ?]]; destruct_and!.
-    exists (dvl (pv (vobj ds'))), g1; split_and!; cbn;
+    exists (dpt (pv (vobj ds'))), g1; split_and!; cbn;
       try eapply typing_stamped.dnew_typed; eauto 2;
       repeat constructor; eauto with f_equal.
   - intros * Hu1 IHs1 Hu2 IHs2 g.
@@ -270,7 +270,7 @@ Section syntyping_stamping_lemmas.
       which holds but would require extra boilerplate. *)
     move: IHs1 => /(.$ g) [g1 [Hts1 Hle1]].
     move: IHs2 => /(.$ g1) [d' [g2 [Hts2 [Hle2 Hs]]]]; lte g g1 g2.
-    have [p' Heq]: ∃ p', d' = dvl p'. {
+    have [p' Heq]: ∃ p', d' = dpt p'. {
       move: Hs => {Hts2}; destruct d'; rewrite /= /from_option => -[?[??]];
         try case_match; simplify_eq; eauto 2.
     }
